lean/Maquina.lean
@@ -7,6 +7,7 @@ import Maquina.Queue
 import Maquina.Process
 import Maquina.Machine
 import Maquina.Operation
+import Maquina.Simulator
 import Maquina.Examples
 
 /-!
